\part{Tables}

\section{Inverse of 3x3 matrix}
\begin{equation}
\left(\begin{array}{ccc}
    a & b & c\\
    d & e & f\\
    g & h &i
\end{array}\right)^{-1}
=
{\frac{1}{\rm{det}}}
\left(\begin{array}{rrr}
    e i - f h & c h - b i & b f - c e\\
    f g - d i & a i - c g & c d - a f\\
    d h - e g & b g - a h & a e - b d
\end{array}\right)
\end{equation}


\section{Trig functions}
\begin{align}
    \cot(\theta) &= \frac{1}{\tan(\theta)}\\
    \sec(\theta) &= \frac{1}{\cos(\theta)}\\
    \csc(\theta) &= \frac{1}{\sin(\theta)}\\
    \sin(\theta) &= \frac{\text{motst√•ende}}{\text{hypotenus}}\\
    \cos(\theta) &= \frac{\text{hosliggende}}{\text{hypotenus}}\\
    \tan(\theta) &= \frac{\sin(\theta)}{\cos(\theta)}
\end{align}

\section{Trig identities}
\begin{align}
    \cos(\theta)\sin(\theta) &= \frac{1}{2}\sin(2\theta)\\
    \cos^2(\theta)-\sin^2(\theta) &= \cos(2\theta)\\
    \sin(\alpha+\beta) &= \sin(\alpha)\cos(\beta) + \cos(\alpha)\sin(\beta)\\
    \cos(\alpha+\beta) &= \cos(\alpha)\cos(\beta) - \sin(\alpha)\sin(\beta)\\
    \sin(\alpha-\beta) &= \sin(\alpha)\cos(\beta) - \cos(\alpha)\sin(\beta)\\
    \cos(\alpha-\beta) &= \cos(\alpha)\cos(\beta) + \sin(\alpha)\sin(\beta)
\end{align}
